Tealeaves/Adapters/CategoricalToKleisli/DecoratedTraversableMonadPoly.v
@@ -1,0 +1,86 @@
+From Tealeaves Require Import
+  Classes.Categorical.DecoratedTraversableMonadPoly
+  Classes.Kleisli.DecoratedTraversableMonadPoly.
+
+#[local] Generalizable Variables T.
+
+(** * Kleisli DTMs from Categorical DTMs *)
+(**********************************************************************)
+
+(** ** Derived Operations *)
+(**********************************************************************)
+Module DerivedOperations.
+
+  #[export] Instance Binddt_Categorical
+    (T: Type -> Type -> Type)
+    `{Map2 T}
+    `{DecoratePoly T}
+    `{ApplicativeDist2 T}
+    `{forall B, Join (T B)}: Substitute T T :=
+    fun (B1 V1 B2 V2: Type)
+      (G : Type -> Type)
+      `{Map_G: Map G} `{Pure_G: Pure G} `{Mult_G: Mult G}
+      (ρ: list B1 * B1 -> G B2) (* rename binders *)
+      (σ: list B1 * V1 -> G (T B2 V2)) (* insert subtrees *)
+    => (map (F := G) join ∘ dist2 (T := T) (G := G) ∘ map2 ρ σ ∘ decp (F := T) (B := B1) (V := V1)).
+
+End DerivedOperations.
+
+Module DerivedInstances.
+
+  Import DerivedOperations.
+
+  Context
+    `{Categorical.DecoratedTraversableMonadPoly.DecoratedTraversableMonadPoly T}.
+
+  Instance: Kleisli.DecoratedTraversableMonadPoly.DecoratedTraversableMonadPoly T.
+  Proof.
+    constructor; intros.
+    - unfold substitute, Binddt_Categorical.
+      reassociate -> on left.
+      rewrite xxx_dec_ret.
+      reassociate <- on left.
+      fequal.
+      reassociate ->.
+      rewrite xxx_map_ret.
+      reassociate <- on left.
+      change σ with (id ∘ σ) at 2.
+      fequal.
+      reassociate -> on left.
+      rewrite (xxx_dist2_ret (G := G) (T := T) (B := B2) (V := T B2 A2)).
+      rewrite fun_map_map.
+      setoid_rewrite mon_join_ret.
+      rewrite fun_map_id.
+      reflexivity.
+    - unfold substitute, Binddt_Categorical.
+      rewrite <- fun2_map21_map2.
+      (* unfold_ops @Map2_1. *)
+      reassociate <-.
+      reassociate -> on left.
+      rewrite dfunp_dec_extract.
+      change (?x ∘ id) with x.
+      rewrite dist2_unit.
+      change (?x ∘ id) with x.
+      unfold_ops Map_I.
+      apply mon_join_map_ret.
+    - unfold substitute.
+      unfold Binddt_Categorical.
+      repeat reassociate <- on left.
+      rewrite fun_map_map.
+      fequal.
+      admit.
+    - unfold substitute.
+      unfold Binddt_Categorical.
+      repeat reassociate <- on left.
+      rewrite appmor_natural_pf.
+      reassociate -> near dist2.
+      unfold compose at 9.
+      rewrite <- (dist2_morph (T := T) (ϕ := ϕ)).
+      reassociate <- on left.
+      reassociate -> near (map2 ρ σ).
+      rewrite fun2_map_map.
+      reflexivity.
+  Admitted.
+
+End DerivedInstances.
+
