Tealeaves/Backends/Named/NamedTraditional.v
@@ -1,0 +1,91 @@
+From Tealeaves Require Import
+  Classes.EqDec_eq
+  Classes.Kleisli.DecoratedTraversableMonadPoly
+  Functors.List_Telescoping_General
+  Backends.Named.Names
+  Backends.Named.Named
+  Functors.Constant
+  Functors.Subset.
+
+Import Subset.Notations.
+Import Monoid.Notations.
+Import Applicative.Notations.
+Import List.ListNotations.
+Import Product.Notations.
+Import ContainerFunctor.Notations.
+
+Section alt.
+
+  Context
+    {T: Type -> Type -> Type}
+    `{forall W, Return (T W)}
+    `{Substitute T T}.
+
+  Import DecoratedTraversableMonadPoly.DerivedOperations.
+
+  Section rename_local.
+
+    Context (conflicts: list name).
+    (* X is the var being substituted, fv_u is FV u *)
+    Context (x: name) (fv_u: list name) (u: T name name).
+
+    (* Given a substitution of x by u, encode the logic of what happens at <<current>> if <<history>> is the set of names
+     given to the binders so far *)
+    Definition rename_binder_local_history:
+      list name * name -> name :=
+      fun '(history, b) =>
+        if x == b
+        then b
+        else if SmartAtom.name_inb b (fv_u)
+             then fresh (conflicts ++ history ++ [b])
+             else b.
+
+    Definition ctx_to_history: list name -> list name :=
+      fold_with_history rename_binder_local_history.
+
+
+    (* Name a binder to something else during substitution *)
+    Definition rename_binder_local:
+      list name * name -> name :=
+      fun '(ctx, b) =>
+        if SmartAtom.name_inb x ctx (* Halt substitution early *)
+        then b
+        else if x == b (* Else check if halt now *)
+             then b
+             else if SmartAtom.name_inb b fv_u (* Else check if need to rename *)
+             then (rename_binder_local_history (ctx_to_history ctx, b))
+             else b.
+
+    Definition subst_local:
+      list name * name -> T name name :=
+      fun '(ctx, v) =>
+        if SmartAtom.name_inb x ctx (* Halt substitution early *)
+        then ret (T := T name) v
+        else
+               match (get_binding ctx v) with
+               | Unbound _ =>
+                   if v == x
+                   then u
+                   else ret (T := T name) v
+               | Bound prefix _ _ =>
+                   if v == x
+                   then ret (T := T name) v
+                   else if SmartAtom.name_inb v (FV T u)
+                        then ret (T := T name) (rename_binder_local_history (prefix, v))
+                        else ret (T := T name) v
+               end.
+
+    Definition subst_top
+      (t: T name name): T name name :=
+      substitute (G := fun A => A) (U := T)
+        rename_binder_local
+        subst_local t.
+
+  End rename_local.
+
+  Definition subst
+    (x: name) (u: T name name)
+    (t: T name name): T name name :=
+    subst_top (FV T t ++ FV T u) x (FV T u) u t.
+
+End alt.
