Tealeaves/Classes/Categorical/DecoratedFunctorPoly.v
@@ -1,0 +1,71 @@
+From Tealeaves Require Export
+  Classes.Categorical.Comonad
+  Functors.Reader
+  Functors.List_Telescoping_General
+  Classes.Functor2
+  Classes.Monoid
+  Functors.Z2.
+
+Import Monoid.Notations.
+
+(** * <<shift2>> *)
+(**********************************************************************)
+Definition shift2 {F: Type -> Type -> Type}
+  `{Map2 F} {W} `{Monoid_op W} {A1 A2} :
+  W * F (W * A1) (W * A2) -> F (W * A1) (W * A2) :=
+  map2 (uncurry incr) (uncurry incr) ∘ strength2.
+
+Lemma map2_shift2_preincr
+  {F: Type -> Type -> Type}
+  `{Map2 F}
+  `{! Functor2 F}
+  {W} `{Monoid_op W}
+  {B1 V1 B2 V2} {g: W * B1 -> B2} {f: W * V1 -> V2} {w: W}:
+  map2 g f ∘ shift2 ∘ pair w = map2 (g ⦿ w) (f ⦿ w).
+Proof.
+  intros.
+  ext t.
+  unfold shift2.
+  unfold compose.
+  unfold strength2.
+  compose near t on left.
+  rewrite (fun2_map_map).
+  compose near t on left.
+  rewrite (fun2_map_map).
+  reflexivity.
+Qed.
+
+(** * Poly Decorated functors *)
+(**********************************************************************)
+
+(** ** Operations *)
+(**********************************************************************)
+Class DecoratePoly
+  (F: Type -> Type -> Type) :=
+  decp: forall (B V: Type), F B V -> F (Z B) (Z2 B V).
+
+#[global] Arguments decp {F}%function_scope {DecoratePoly}
+  {B V}%type_scope _.
+
+#[local] Arguments decp {F}%function_scope {DecoratePoly}
+  {B V}%type_scope _.
+
+Definition PolyDecorateNatural F `{Map2 F} `{DecoratePoly F}: Prop :=
+  forall (B V B' V': Type) (g: B -> B') (f: V -> V'),
+    decp (B := B') (V := V') ∘ map2 g f =
+      map2 (map (F := Z) g) (map2 (F := Z2) g f) ∘ decp (B := B) (V := V).
+
+
+(** ** Typeclass *)
+(**********************************************************************)
+Class DecoratedFunctorPoly
+  (F: Type -> Type -> Type)
+  `{Map2 F}
+  `{DecoratePoly F} :=
+  { dfunp_functor :> Functor2 F;
+    dfunp_natural: PolyDecorateNatural F;
+    dfunp_dec_dec: forall (B V: Type),
+      decp ∘ decp (B := B) (V := V) = map2 (cojoin (W := Z)) cojoin_Z2 ∘ decp;
+    dfunp_dec_extract: forall (B V: Type),
+      map2 (extract) (extract) ∘ decp (B := B) (V := V) = @id (F B V);
+  }.
