Tealeaves/Classes/Categorical/DecoratedTraversableMonadPoly.v
@@ -1,0 +1,89 @@
+From Tealeaves Require Export
+  Classes.Categorical.DecoratedFunctorPoly
+  Classes.Categorical.TraversableFunctor2
+  Classes.Categorical.ApplicativeCommutativeIdempotent
+  Classes.Categorical.Monad
+  Functors.List
+  Functors.Writer.
+
+#[local] Generalizable Variables T F G W A B C.
+
+Section laws.
+
+  Context (T: Type -> Type -> Type).
+
+  Context
+    `{Map2 T} `{DecoratePoly T} `{ApplicativeDist2 T}
+    `{forall B, Return (T B)}
+    `{forall B, Join (T B)}.
+
+  Definition decpoly_ret: Prop :=
+    forall {B V: Type},
+      decp ∘ ret (T := T B) (A := V) =
+        ret (T := T (Z B)) (A := Z2 B V) ∘ ret (T := prod (list B)).
+
+  Definition decpoly_join: Prop :=
+    forall {B V: Type},
+      decp ∘ join (T := T B) (A := V) =
+        join (T := T (Z B)) ∘ map2 id (shift2 ∘ map_snd decp)
+          ∘ decp (B := B) (V := T B V).
+
+  Definition dist2_join: Prop :=
+    forall {B V: Type} `{Applicative G},
+      dist2 ∘ join (T := T (G B)) (A := (G V)) =
+        map (F := G) (join (T := T B)) ∘
+          dist2 (T := T) (G := G) ∘
+          map2 (F := T) id (dist2).
+
+  Definition dist2_ret: Prop :=
+    forall {B V: Type} `{Applicative G},
+      dist2 ∘ ret (T := T (G B)) (A := G V) =
+        map (F := G) (ret (T := T B) (A := V)).
+
+
+  Definition dist2_decpoly_ci: Prop :=
+    forall (B V: Type) `{ApplicativeCommutativeIdempotent G},
+      dist2 (G := G) ∘ map2 (dist Z G) (dist2 (T := Z2)) ∘ (decp (B := G B) (V := G V)) =
+        map (F := G) (decp (B := B) (V := V)) ∘ dist2 (T := T) (G := G).
+
+End laws.
+
+(** * Decorated-traversable monads *)
+(**********************************************************************)
+Class DecoratedTraversableMonadPoly
+  (T: Type -> Type -> Type)
+  `{Map2 T} `{DecoratePoly T} `{ApplicativeDist2 T}
+  `{forall B, Return (T B)}
+  `{forall B, Join (T B)} :=
+  {
+    xxx_functor :> Functor2 T;
+    xxx_decorated :> DecoratedFunctorPoly T;
+    xxx_traversable :> TraversableFunctor2 T;
+    xxx_monad :> forall B, Monad (T B);
+    xxx_map_ret: forall B B' V V' (g: B -> B') (f: V -> V'),
+      map2 g f ∘ ret (T := T B) (A := V) =
+        ret (T := T B') (A := V') ∘ f;
+    xxx_dec_ret: forall B V,
+      decp ∘ ret (T := T B) (A := V) =
+        ret (T := T (Z B)) (A := Z2 B V) ∘ ret (T := prod (list B));
+    xxx_dec_join:
+    forall {B V: Type},
+      decp ∘ join (T := T B) (A := V) =
+        join (T := T (Z B)) ∘ map2 id (shift2 ∘ map_snd decp)
+          ∘ decp (B := B) (V := T B V);
+    xxx_dist2_ret:
+    forall {B V: Type} `{Applicative G},
+      dist2 ∘ ret (T := T (G B)) (A := G V) =
+        map (F := G) (ret (T := T B) (A := V));
+    xxx_dist2_join:
+    forall {B V: Type} `{Applicative G},
+      dist2 ∘ join (T := T (G B)) (A := (G V)) =
+        map (F := G) (join (T := T B)) ∘
+          dist2 (T := T) (G := G) ∘
+          map2 (F := T) id (dist2);
+    xxx_dist2_decpoly:
+    forall (B V: Type) `{ApplicativeCommutativeIdempotent G},
+      dist2 (G := G) ∘ map2 (dist Z G) (dist2 (T := Z2)) ∘ (decp (B := G B) (V := G V)) =
+        map (F := G) (decp (B := B) (V := V)) ∘ dist2 (T := T) (G := G);
+  }.
+
