Tealeaves/Examples/Lambda/Autosubst.v
@@ -1,0 +1,18 @@
+(* Require the Autosubst library *)
+From Autosubst Require Import Autosubst.
+
+
+Inductive term: Type :=
+| tvar (x: var)
+| tapp (t1 t2: term)
+| tabs (t: {bind term}).
+
+Instance Ids_term: Ids term. Proof. derive. Defined.
+Instance Rename_term: Rename term. Proof. derive. Defined.
+Instance Subst_term: Subst term. Proof. derive. Defined.
+Instance SubstLemmas_term: SubstLemmas term. derive. Qed.
+
+Print SubstLemmas.
+
+Instance substLemmas_term: SubstLemmas term.
+Proof. apply SubstLemmas_Ind; intros; simpl; congruence. Qed.
