Tealeaves/Examples/LambdaNominal/Categorical.v
@@ -1,0 +1,970 @@
+From Tealeaves Require Export
+  Examples.LambdaNominal.Syntax
+  Classes.Categorical.DecoratedMonad (shift).
+
+#[local] Generalizable Variables G.
+
+(*|
+============================================
+Decomposition into categorical components
+============================================
+|*)
+
+(*|
++++++++++++++++++++++++++++++++++++++++++++++++
+Map
++++++++++++++++++++++++++++++++++++++++++++++++
+|*)
+Fixpoint map2_term {B1 V1 B2 V2: Type} (ρ: B1 -> B2) (σ: V1 -> V2)
+  (t: term B1 V1): term B2 V2 :=
+  match t with
+  | tvar v => (@tvar B2 V2) (σ v)
+  | lam v body => lam (ρ v) (map2_term ρ σ body)
+  | tap t1 t2 => tap (map2_term ρ σ t1) (map2_term ρ σ t2)
+  end.
+
+Lemma map2_id_term: forall (B1 V1: Type),
+    map2_term (@id B1) (@id V1) = @id (term B1 V1).
+Proof.
+  intros. ext t. induction t.
+  - reflexivity.
+  - cbn. now rewrite IHt.
+  - cbn. now rewrite IHt1, IHt2.
+Qed.
+
+Lemma map2_map2_term: forall (B1 V1 B2 V2 b3 v3: Type)
+                      (ρ1: B1 -> B2) (σ1: V1 -> V2) (ρ2: B2 -> b3) (σ2: V2 -> v3),
+    map2_term ρ2 σ2 ∘ map2_term ρ1 σ1 = map2_term (ρ2 ∘ ρ1) (σ2 ∘ σ1).
+Proof.
+  intros. ext t. induction t.
+  - reflexivity.
+  - cbn. compose near t on left. now rewrite IHt.
+  - cbn.
+    compose near t1 on left. rewrite IHt1.
+    compose near t2 on left. rewrite IHt2.
+    reflexivity.
+Qed.
+
+#[export] Instance Map2_term: Map2 term.
+Proof.
+  intros A1 B1 A2 B2 f1 f2.
+  apply (map2_term f1 f2).
+Defined.
+
+Section map_term_rewriting.
+
+  Context
+    {B1 V1 B2 V2: Type}
+      (ρ: B1 -> B2)
+      (σ: V1 -> V2).
+
+  Lemma map2_term_rw1: forall (v: V1),
+      map2 ρ σ (tvar (B := B1) v) = tvar (σ v).
+  Proof.
+    reflexivity.
+  Qed.
+
+  Lemma map2_term_rw2: forall (b: B1) (body: term B1 V1),
+      map2 ρ σ (lam b body) = lam (ρ b) (map2 ρ σ body).
+  Proof.
+    reflexivity.
+  Qed.
+
+  Lemma map2_term_rw3: forall (t1 t2: term B1 V1),
+      map2 ρ σ (tap t1 t2) = tap (map2 ρ σ t1) (map2 ρ σ t2).
+  Proof.
+    reflexivity.
+  Qed.
+
+End map_term_rewriting.
+
+
+#[export] Instance Functor2_term: Functor2 term.
+Proof.
+  constructor.
+  - intros. ext t. induction t.
+    + reflexivity.
+    + rewrite map2_term_rw2.
+      now rewrite IHt.
+    + rewrite map2_term_rw3.
+      rewrite IHt1.
+      rewrite IHt2.
+      reflexivity.
+  - intros. unfold compose. ext t.
+    induction t.
+    + reflexivity.
+    + rewrite map2_term_rw2.
+      rewrite map2_term_rw2.
+      rewrite IHt.
+      reflexivity.
+    + rewrite map2_term_rw3.
+      rewrite map2_term_rw3.
+      rewrite IHt1.
+      rewrite IHt2.
+      reflexivity.
+Defined.
+
+(*|
++++++++++++++++++++++++++++++++++++++++++++++++
+Decoration
++++++++++++++++++++++++++++++++++++++++++++++++
+|*)
+
+Fixpoint dec_term_rec {B V: Type} (ctx: list B)
+  (t: term B V): term (list B * B) (list B * V) :=
+  match t with
+  | tvar v => tvar (ctx, v)
+  | lam b body => lam (ctx, b) (dec_term_rec (ctx ++ [b]) body)
+  | tap t1 t2 => tap (dec_term_rec ctx t1) (dec_term_rec ctx t2)
+  end.
+
+Definition dec_term {B V: Type}:
+  term B V ->
+  term (list B * B) (list B * V) :=
+  dec_term_rec nil.
+
+Lemma dec_term_shift1 {B V: Type}:
+  forall (ctx1 ctx2: list B) (t: term B V),
+    dec_term_rec (ctx1 ++ ctx2) t =
+      shift2 (ctx1, dec_term_rec ctx2 t).
+Proof.
+  intros.
+  generalize dependent ctx1.
+  generalize dependent ctx2.
+  induction t; intros.
+  - cbn.
+    reflexivity.
+  - cbn.
+    fequal.
+    rewrite <- List.app_assoc.
+    rewrite IHt.
+    compose near (dec_term_rec (ctx2 ++ [b]) t).
+    rewrite (fun2_map_map).
+    rewrite IHt.
+    unfold shift2.
+    unfold compose at 6.
+    compose near (strength2 (ctx2, dec_term_rec [b] t)).
+    rewrite fun2_map_map.
+    unfold compose at 3.
+    cbn.
+    compose near ((map2 (pair ctx2) (pair ctx2) (dec_term_rec [b] t))) on left.
+    rewrite fun2_map_map.
+    compose near ((map2 (pair ctx2) (pair ctx2) (dec_term_rec [b] t))) on left.
+    rewrite fun2_map_map.
+    fequal.
+  - cbn.
+    rewrite IHt1.
+    rewrite IHt2.
+    reflexivity.
+Qed.
+
+Lemma dec_term_shift {B V: Type}:
+  forall (ctx: list B) (t: term B V),
+    dec_term_rec ctx t =
+      shift2 (ctx, dec_term t).
+Proof.
+  intros.
+  rewrite <- (List.app_nil_r ctx) at 1.
+  rewrite dec_term_shift1.
+  reflexivity.
+Qed.
+
+#[export] Instance: DecoratePoly term := @dec_term.
+
+Section dec_term_rewriting.
+
+  Context (B V: Type) (ctx: list B).
+
+  Lemma dec_term_rec_rw1: forall (v: V),
+      dec_term_rec ctx (tvar v) = tvar (ctx, v).
+  Proof.
+    reflexivity.
+  Qed.
+
+  Lemma dec_term_rec_rw2: forall (b: B) (body: term B V),
+      dec_term_rec ctx (lam b body) =
+        lam (ctx, b) (dec_term_rec (ctx ++ [b]) body).
+  Proof.
+    reflexivity.
+  Qed.
+
+  Lemma dec_term_rec_rw3: forall (t1 t2: term B V),
+      dec_term_rec ctx (tap t1 t2) = tap (dec_term_rec ctx t1) (dec_term_rec ctx t2).
+  Proof.
+    reflexivity.
+  Qed.
+
+  Lemma dec_term_rw1: forall (v: V),
+      decp (tvar (B := B) v) = tvar ([], v).
+  Proof.
+    cbn.
+    reflexivity.
+  Qed.
+
+  Lemma dec_term_rw2: forall (b: B) (body: term B V),
+      decp (lam b body) = lam ([], b) (shift2 ([b], decp body)).
+  Proof.
+    intros. cbn.
+    rewrite dec_term_shift.
+    reflexivity.
+  Qed.
+
+  Lemma dec_term_rw2': forall (b: B) (body: term B V),
+      decp (lam b body) = lam ([], b) (dec_term_rec [b] body).
+  Proof.
+    reflexivity.
+  Qed.
+
+  Lemma dec_term_rw3: forall (t1 t2: term B V),
+      decp (tap t1 t2) = tap (decp t1) (decp t2).
+  Proof.
+    reflexivity.
+  Qed.
+
+End dec_term_rewriting.
+
+(* Naturality, rec case *)
+Lemma map_dec_rec:
+  forall (B1 V1 B2 V2: Type)
+    (ρ: list B1 * B1 -> B2) (σ: list B1 * V1 -> V2) (ctx: list B1),
+    map2 ρ σ ∘ dec_term_rec ctx =
+      map2 (ρ ⦿ ctx) (σ ⦿ ctx) ∘ dec_term.
+Proof.
+  intros. ext t. unfold compose.
+  generalize dependent ctx.
+  generalize dependent σ.
+  generalize dependent ρ.
+  induction t; intros ρ σ ctx.
+  - cbn. unfold preincr, compose, incr.
+    change (@nil B1) with (Ƶ: list B1).
+    rewrite monoid_id_l.
+    reflexivity.
+  - cbn.
+    rewrite IHt.
+    rewrite IHt.
+    fequal.
+    + unfold preincr, incr, compose, monoid_op, Monoid_op_list.
+      rewrite List.app_nil_r.
+      reflexivity.
+    + rewrite preincr_preincr.
+      rewrite preincr_preincr.
+      reflexivity.
+  - cbn.
+    rewrite IHt1.
+    rewrite IHt2.
+    reflexivity.
+Qed.
+
+Lemma dec_rec_spec:
+  forall (B V: Type) (ctx: list B),
+    dec_term_rec ctx =
+      map2 (incr ctx) (incr ctx) ∘ dec_term (V := V).
+Proof.
+  intros.
+  change_left (id ∘ dec_term_rec ctx (V := V)).
+  rewrite <- fun2_map_id.
+  rewrite map_dec_rec.
+  reflexivity.
+Qed.
+
+(* Counit law *)
+Lemma dec_rec_extract_term: forall (B V: Type) (ctx: list B),
+    map2 (extract_Z2) (extract_Z2) ∘ dec_term_rec ctx = @id (term B V).
+Proof.
+  intros. ext t. unfold compose.
+  generalize dependent ctx. induction t; intro ctx.
+  - reflexivity.
+  - cbn. now rewrite IHt.
+  - cbn. now rewrite IHt1, IHt2.
+Qed.
+
+Lemma dec_extract_term: forall (B V: Type),
+    map2 (extract_Z2) (extract_Z2) ∘ dec_term = @id (term B V).
+Proof.
+  intros. unfold dec_term. apply dec_rec_extract_term.
+Qed.
+
+(* cojoin law *)
+Lemma dec_rec_dec_rec_term: forall (B V: Type) (ctx: list B),
+    dec_term_rec (decorate_prefix_list ctx) ∘ dec_term_rec ctx =
+      map2 (cojoin_Z2) (cojoin_Z2) ∘ dec_term_rec ctx (B := B) (V := V).
+Proof.
+  intros. ext t. unfold compose.
+  generalize dependent ctx.
+  induction t; intro ctx.
+  - reflexivity.
+  - cbn.
+    rewrite <- IHt.
+    rewrite decorate_prefix_list_rw_app.
+    cbn. change (@nil B) with (Ƶ: list B).
+    rewrite monoid_id_l.
+    reflexivity.
+  - cbn. now rewrite IHt1, IHt2.
+Qed.
+
+Lemma dec_dec_term: forall (B V: Type),
+    dec_term ∘ dec_term (B := B) (V := V) =
+      map2 (cojoin_Z2) (cojoin_Z2) ∘ dec_term.
+Proof.
+  intros. unfold dec_term.
+  change (@nil (list B * B)) with (decorate_prefix_list (@nil B)).
+  apply dec_rec_dec_rec_term.
+Qed.
+
+Section naturality.
+
+  Context {B1 V1 B2 V2: Type}
+    (ρ: B1 -> B2) (σ: V1 -> V2).
+
+  Lemma dec_rec_map: forall (ctx: list B1),
+      dec_term_rec (map ρ ctx) ∘ map2 ρ σ =
+        map2 (map_pair (map (F := list) ρ) ρ)
+          (map_pair (map (F := list) ρ) σ) ∘ dec_term_rec ctx.
+  Proof.
+    intros. ext t. unfold compose.
+    generalize dependent ρ; clear ρ.
+    generalize dependent σ; clear σ.
+    generalize dependent ctx.
+    induction t as [v | b body IHbody | t1 IHt1 t2 IHt2];
+      intros.
+    - reflexivity.
+    - cbn.
+      fequal.
+      replace (map ρ ctx ++ [ρ b])
+        with (map ρ (ctx ++ [b])) by now rewrite map_list_app.
+      rewrite IHbody.
+      reflexivity.
+    - cbn.
+      rewrite IHt1.
+      rewrite IHt2.
+      reflexivity.
+  Qed.
+
+  Lemma dec_map:
+    dec_term ∘ map2 ρ σ =
+      map2 (map_pair (map (F := list) ρ) ρ)
+        (map_pair (map (F := list) ρ) σ) ∘ dec_term.
+  Proof.
+    unfold dec_term.
+    change (@nil B2) with (map ρ nil).
+    rewrite dec_rec_map.
+    reflexivity.
+  Qed.
+
+End naturality.
+
+#[export] Instance: DecoratedFunctorPoly term.
+Proof.
+  constructor.
+  - typeclasses eauto.
+  - unfold PolyDecorateNatural.
+    intros.
+    setoid_rewrite dec_map.
+    fequal.
+    fequal.
+    now ext [ctx a].
+  - intros.
+    rewrite dec_dec_term.
+    reflexivity.
+  - intros.
+    rewrite dec_extract_term.
+    reflexivity.
+Qed.
+
+
+(*|
++++++++++++++++++++++++++++++++++++++++++++++++
+Applicative distribution
++++++++++++++++++++++++++++++++++++++++++++++++
+|*)
+
+Fixpoint dist_term
+  {G: Type -> Type} `{Map G} `{Pure G} `{Mult G}
+   {B V: Type}
+  (t: term (G B) (G V)): G (term B V) :=
+  match t with
+  | tvar vr => map (@tvar B V) vr
+  | lam bin body => pure (@lam B V)
+                     <⋆> bin
+                     <⋆> dist_term body
+  | tap t1 t2 => pure (@tap B V)
+                  <⋆> dist_term t1
+                  <⋆> dist_term t2
+  end.
+
+#[export] Instance term_dist2: ApplicativeDist2 term := @dist_term.
+
+Lemma dist_term_morph:
+  forall (G1 G2 : Type -> Type)
+    `{Map G1} `{Mult G1} `{Pure G1}
+    `{Map G2} `{Mult G2} `{Pure G2}
+    (ϕ: forall (A: Type), G1 A -> G2 A),
+    ApplicativeMorphism G1 G2 ϕ ->
+    forall (B V: Type),
+      dist2 (G := G2) ∘ map2 (ϕ B) (ϕ V) =
+
+        ϕ (term B V) ∘ dist2 (G := G1) (B := B) (A := V).
+Proof.
+  intros. ext t. unfold compose.
+  induction t.
+  - cbn.
+    rewrite appmor_natural.
+    reflexivity.
+  - cbn.
+    rewrite IHt.
+    rewrite ap_morphism_1.
+    rewrite ap_morphism_1.
+    rewrite appmor_pure.
+    reflexivity.
+  - cbn.
+    rewrite IHt1.
+    rewrite IHt2.
+    rewrite ap_morphism_1.
+    rewrite ap_morphism_1.
+    rewrite appmor_pure.
+    reflexivity.
+Qed.
+
+Lemma dist_term_linear:
+  forall (G1 G2 : Type -> Type)
+    `{Map G1} `{Mult G1} `{Pure G1} `{! Applicative G1}
+    `{Map G2} `{Mult G2} `{Pure G2} `{! Applicative G2},
+  forall (B V: Type),
+    dist2 (G := G1 ∘ G2) =
+    map (F := G1) (dist2 (G := G2)) ∘
+      dist2 (T := term) (G := G1) (B := G2 B) (A := G2 V).
+Proof.
+  intros. ext t. unfold compose at 4.
+  induction t.
+  - cbn. compose near v on right.
+    rewrite fun_map_map.
+    reflexivity.
+  - cbn.
+    rewrite IHt.
+    unfold_ops @Pure_compose.
+    rewrite (ap_compose2 G2 G1).
+    rewrite (ap_compose2 G2 G1).
+    rewrite map_ap.
+    rewrite app_pure_natural.
+    rewrite app_pure_natural.
+    rewrite <- ap_map.
+    rewrite map_ap.
+    rewrite app_pure_natural.
+    rewrite map_ap.
+    rewrite map_ap.
+    rewrite app_pure_natural.
+    reflexivity.
+  - cbn.
+    rewrite IHt1.
+    rewrite IHt2.
+    unfold_ops @Pure_compose.
+    rewrite (ap_compose2 G2 G1).
+    rewrite (ap_compose2 G2 G1).
+    rewrite map_ap.
+    rewrite map_ap.
+    rewrite map_ap.
+    rewrite app_pure_natural.
+    rewrite app_pure_natural.
+    rewrite app_pure_natural.
+    rewrite <- ap_map.
+    rewrite map_ap.
+    rewrite app_pure_natural.
+    rewrite <- ap_map.
+    rewrite app_pure_natural.
+    reflexivity.
+Qed.
+
+Section naturality.
+
+  Context {B1 V1 B2 V2: Type}
+    (ρ: B1 -> B2) (σ: V1 -> V2).
+
+  Lemma dist_map `{Applicative G}:
+    map (map2 ρ σ) ∘ dist_term (G := G) =
+      dist_term ∘ map2 (map ρ) (map σ).
+  Proof.
+    intros. ext t. unfold compose.
+    induction t as [v | b body IHbody | t1 IHt1 t2 IHt2];
+      change (@nil B2) with (map ρ nil).
+    - cbn.
+      compose near v on left.
+      rewrite fun_map_map.
+      compose near v on right.
+      rewrite fun_map_map.
+      reflexivity.
+    - cbn.
+      rewrite map_ap.
+      rewrite map_ap.
+      rewrite app_pure_natural.
+      rewrite <- ap_map.
+      rewrite app_pure_natural.
+      rewrite <- IHbody.
+      rewrite <- ap_map.
+      rewrite map_ap.
+      rewrite app_pure_natural.
+      reflexivity.
+    - cbn.
+      rewrite map_ap.
+      rewrite map_ap.
+      rewrite app_pure_natural.
+      rewrite <- IHt1.
+      rewrite <- ap_map.
+      rewrite app_pure_natural.
+      rewrite <- IHt2.
+      rewrite <- ap_map.
+      rewrite map_ap.
+      rewrite app_pure_natural.
+      reflexivity.
+  Qed.
+
+
+End naturality.
+
+#[export] Instance Natural_dist2_term:
+  forall (G : Type -> Type) (Map_G : Map G) (Pure_G : Pure G) (Mult_G : Mult G),
+    Applicative G -> Natural2 (@dist2 term term_dist2 G Map_G Pure_G Mult_G).
+Proof.
+  intros.
+  constructor.
+  - typeclasses eauto.
+  - typeclasses eauto.
+  - intros. apply dist_map.
+    auto.
+Qed.
+
+#[export] Instance TraversableFunctor2_term: TraversableFunctor2 term.
+Proof.
+  constructor.
+  - typeclasses eauto.
+  - typeclasses eauto.
+  - apply dist_term_morph.
+  - intros. ext t. unfold id. induction t.
+    reflexivity.
+    cbn. rewrite IHt. reflexivity.
+    cbn. rewrite IHt1, IHt2. reflexivity.
+  - intros. apply dist_term_linear; auto.
+Qed.
+
+(*|
++++++++++++++++++++++++++++++++++++++++++++++++
+Join
++++++++++++++++++++++++++++++++++++++++++++++++
+|*)
+
+Fixpoint join_term {B V: Type} (t: term B (term B V)): term B V :=
+  match t with
+  | tvar v => v
+  | lam b body => lam b (join_term body)
+  | tap t1 t2 => tap (join_term t1) (join_term t2)
+  end.
+
+Lemma join_ret_term {B V: Type}:
+  join_term ∘ ret (A := term B V) = @id (term B V).
+Proof.
+  reflexivity.
+Qed.
+
+Lemma join_map_ret_term {B V: Type}:
+  join_term ∘ map2 (@id B) (ret (A := V)) = @id (term B V).
+Proof.
+  ext t. unfold compose. induction t.
+  - reflexivity.
+  - cbn. rewrite IHt. reflexivity.
+  - cbn. rewrite IHt1, IHt2. reflexivity.
+Qed.
+
+Lemma join_join_term {B V: Type}:
+  join_term ∘ join_term (B := B) (V := term B V) =
+    join_term ∘ map2 id (join_term).
+Proof.
+  intros. ext t.
+  unfold compose.
+  induction t as [v | b body IHbody | t1 IHt1 t2 IHt2].
+  - reflexivity.
+  - cbn.
+    rewrite IHbody.
+    reflexivity.
+  - cbn.
+    rewrite IHt1.
+    rewrite IHt2.
+    reflexivity.
+Qed.
+
+#[export] Instance Join_lambda_term: forall B, Join (term B) :=
+  @join_term.
+
+Section join_term_rewriting.
+
+  Context (B V: Type).
+
+  Lemma join_term_rw1: forall (v: term B V),
+      join (tvar (B := B) v) = v.
+  Proof.
+    reflexivity.
+  Qed.
+
+  Lemma join_term_rw2: forall (b: B) (body: term B (term B V)),
+      join (lam b body) = lam b (join body).
+  Proof.
+    reflexivity.
+  Qed.
+
+  Lemma join_term_rw3: forall (t1 t2: term B (term B V)),
+      join (tap t1 t2) = tap (join t1) (join t2).
+  Proof.
+    reflexivity.
+  Qed.
+
+End join_term_rewriting.
+
+Section naturality.
+
+  Context {B1 V1 B2 V2: Type}
+    (ρ: B1 -> B2) (σ: V1 -> V2).
+
+  Lemma join_map:
+    join (T := term B2) ∘ map2 ρ (map2 ρ σ) =
+      map2 ρ σ ∘ (join (T := term B1) (A := V1)).
+  Proof.
+    ext t. unfold compose.
+    induction t as [v | b body IHbody | t1 IHt1 t2 IHt2].
+    - reflexivity.
+    - cbn.
+      rewrite IHbody.
+      reflexivity.
+    - cbn.
+      rewrite IHt1.
+      rewrite IHt2.
+      reflexivity.
+  Qed.
+
+End naturality.
+
+Instance Monad_term: forall B, Monad (term B).
+Proof.
+  constructor.
+  - typeclasses eauto.
+  - constructor; try typeclasses eauto.
+    intros. reflexivity.
+  - constructor; try typeclasses eauto.
+    intros. unfold map, Map2_1.
+    rewrite <- join_map.
+    reflexivity.
+  - intros. reflexivity.
+  - intros. unfold map, Map2_1.
+    apply join_map_ret_term.
+  - intros. unfold map, Map2_1.
+    apply join_join_term.
+Qed.
+
+(*|
++++++++++++++++++++++++++++++++++++++++++++++++
+Distribution and Decoration
++++++++++++++++++++++++++++++++++++++++++++++++
+|*)
+Lemma dist_dec_rec_commute:
+  forall (B V: Type)
+    `{ApplicativeCommutativeIdempotent G}
+    (ctx: list (G B))
+    (t: term (G B) (G V)),
+    dist2 (T := term) (G := G) (map2 dist_Z dist2_Z2 (dec_term_rec ctx t)) =
+      pure (dec_term_rec (B := B) (V := V)) <⋆> (dist list G ctx)
+        <⋆> (dist2 (T := term) (G := G) t).
+Proof.
+  intros.
+  generalize dependent ctx.
+  induction t; intro ctx.
+  - cbn.
+    (* LHS *)
+    rewrite map_ap.
+    rewrite map_ap.
+    rewrite app_pure_natural.
+    (* RHS *)
+    rewrite map_to_ap.
+    rewrite <- ap4.
+    rewrite <- ap4.
+    rewrite ap2.
+    rewrite ap2.
+    rewrite ap3.
+    rewrite <- ap4.
+    rewrite ap2.
+    rewrite ap2.
+    reflexivity.
+  - cbn.
+    (* LHS *)
+    rewrite <- ap4.
+    rewrite ap2.
+    rewrite <- ap4.
+    rewrite ap2.
+    rewrite ap2.
+    rewrite IHt.
+    rewrite <- ap4.
+    rewrite <- ap4.
+    rewrite <- ap4.
+    rewrite ap2.
+    rewrite ap2.
+    rewrite <- ap4.
+    rewrite ap2.
+    rewrite <- ap4.
+    rewrite ap2.
+    rewrite ap2.
+    rewrite ap3.
+    rewrite <- ap4.
+    rewrite ap2.
+    rewrite <- ap4.
+    rewrite ap2.
+    rewrite ap2.
+    rewrite dist_list_app.
+    rewrite <- ap4.
+    rewrite <- ap4.
+    rewrite <- ap4.
+    rewrite ap2.
+    rewrite ap2.
+    rewrite <- ap4.
+    rewrite ap2.
+    rewrite <- ap4.
+    rewrite ap2.
+    rewrite ap2.
+    rewrite ap3.
+    rewrite <- ap4.
+    rewrite ap2.
+    rewrite <- ap4.
+    rewrite ap2.
+    rewrite ap2.
+    rewrite dist_list_one.
+    rewrite <- ap_map.
+    rewrite map_ap.
+    rewrite map_ap.
+    rewrite map_ap.
+    rewrite app_pure_natural.
+    rewrite (ap_flip_x3 (lhs := b) (rhs := dist list G ctx)).
+    rewrite app_pure_natural.
+    rewrite ap_contract.
+    rewrite map_ap.
+    rewrite map_ap.
+    rewrite app_pure_natural.
+    rewrite ap_contract.
+    rewrite app_pure_natural.
+    (* RHS *)
+    rewrite <- ap4.
+    rewrite <- ap4.
+    rewrite <- ap4.
+    rewrite ap2.
+    rewrite ap2.
+    rewrite <- ap4.
+    rewrite ap2.
+    rewrite ap2.
+    rewrite ap3.
+    rewrite <- ap4.
+    rewrite ap2.
+    rewrite ap2.
+    reflexivity.
+  - cbn.
+    rewrite IHt1.
+    rewrite IHt2.
+    rewrite <- ap4; repeat rewrite ap2.
+    rewrite <- ap4; repeat rewrite ap2.
+    rewrite <- ap4; repeat rewrite ap2.
+    rewrite <- ap4; repeat rewrite ap2.
+    rewrite <- ap4; repeat rewrite ap2.
+    rewrite <- ap4; repeat rewrite ap2.
+    rewrite <- ap4; repeat rewrite ap2.
+    (* RHS *)
+    rewrite <- ap4; repeat rewrite ap2.
+    rewrite <- ap4; repeat rewrite ap2.
+    rewrite <- ap4; repeat rewrite ap2.
+    rewrite ap3.
+    rewrite <- ap4; repeat rewrite ap2.
+    rewrite <- ap4; repeat rewrite ap2.
+    rewrite (ap_flip_x3 (G := G)
+               (lhs := dist2 (T := term) (G := G) t1)
+               (rhs := dist list G ctx)).
+    rewrite app_pure_natural.
+    rewrite ap_contract.
+    rewrite app_pure_natural.
+    rewrite ap3.
+    rewrite <- ap4; repeat rewrite ap2.
+    reflexivity.
+Qed.
+
+Lemma dist_dec_commute:
+  forall (B V: Type)
+    `{ApplicativeCommutativeIdempotent G}
+    (t: term (G B) (G V)),
+    dist2 (T := term) (G := G) (map2 dist_Z dist2_Z2 (dec_term t)) =
+      pure (dec_term (B := B) (V := V)) <⋆> (dist2 (T := term) (G := G) t).
+Proof.
+  intros.
+  unfold dec_term.
+  rewrite dist_dec_rec_commute; auto.
+  rewrite dist_list_nil.
+  rewrite ap2.
+  reflexivity.
+Qed.
+
+Lemma dist_dec_commute2:
+  forall (B V: Type)
+    `{ApplicativeCommutativeIdempotent G},
+    dist2 (T := term) (G := G) ∘ map2 (dist_Z (G := G)) (dist2_Z2 (G := G)) ∘ dec_term =
+      map (dec_term (B := B) (V := V)) ∘
+        (dist2 (T := term) (G := G) (B := B) (A := V)).
+Proof.
+  intros.
+  ext t.
+  unfold compose.
+  rewrite dist_dec_commute; auto.
+  rewrite <- map_to_ap.
+  reflexivity.
+Qed.
+
+Lemma dist_dec_rec_commute_map:
+  forall (B1 V1 B2 V2: Type)
+    `{Applicative G}
+    (ctx: list (G B1))
+    (t: term (G B1) (G V1))
+    (ρ: list B1 * B1 -> G B2)
+    (σ: list B1 * V1 -> G V2),
+    True.
+Proof.
+  intros.
+  (*
+  Check
+    (map_term dist_pair dist_pair
+       (dec_term_rec ctx
+          (map_term ρ σ t)).
+    dist2 (map_term dist_pair dist_pair (dec_term_rec ctx t)) =
+      pure (dec_term_rec (B := B1) (V := V1)) <⋆> (dist list G ctx)
+        <⋆> (dist2 t).
+   *)
+Abort.
+
+(*|
++++++++++++++++++++++++++++++++++++++++++++++++
+Join and Decoration
++++++++++++++++++++++++++++++++++++++++++++++++
+|*)
+Lemma decorate_ret_term: forall (B V: Type) (V: V),
+    dec_term (ret (T := term B) V) =
+      ret ([], V).
+Proof.
+  reflexivity.
+Qed.
+
+Lemma decorate_rec_join_term: forall (B V: Type) (ctx: list B),
+    dec_term_rec ctx ∘ join (T := term B) (A := V) =
+      join (T := term (list B * B))
+        ∘ map2 id (shift2 ∘ map_snd dec_term)
+        ∘ dec_term_rec ctx.
+Proof.
+  intros. ext t. unfold compose at 1 2 3.
+  generalize dependent ctx.
+  induction t as [v | b body IHbody | t1 IHt1 t2 IHt2 ]; intro ctx.
+  - (* LHS *)
+    rewrite join_term_rw1.
+    rewrite dec_rec_spec.
+    (* RHS *)
+    rewrite dec_term_rec_rw1.
+    unfold compose at 2.
+    rewrite map2_term_rw1.
+    rewrite join_term_rw1.
+    cbn.
+    compose near (dec_term v) on right.
+    unfold map2, Map2_term.
+    rewrite (map2_map2_term).
+    reflexivity.
+  - cbn.
+    fequal.
+    rewrite IHbody.
+    reflexivity.
+  - cbn.
+    rewrite IHt1.
+    rewrite IHt2.
+    reflexivity.
+Qed.
+
+Lemma decorate_join_term: forall (B V: Type),
+    dec_term ∘ join (T := term B) (A := V) =
+      join (T := term (list B * B)) ∘ map2 id (shift2 ∘ map_snd dec_term)
+        ∘ dec_term.
+Proof.
+  intros.
+  unfold dec_term.
+  rewrite decorate_rec_join_term.
+  reflexivity.
+Qed.
+
+(*|
++++++++++++++++++++++++++++++++++++++++++++++++
+Distribute and Join
++++++++++++++++++++++++++++++++++++++++++++++++
+|*)
+
+(* (t: term (G B) (term (G B) (G V))) *)
+Lemma dist_join_term {B V: Type}
+  `{Applicative G}:
+    dist2 (T := term) (G := G) ∘ join (T := term (G B)) (A := (G V)) =
+      map (F := G) join ∘ dist2 (T := term) (G := G)
+        ∘ map2 (F := term) id (dist2 (T := term) (G := G)).
+Proof.
+  intros. ext t. unfold compose.
+  induction t as [v | b body IHbody | t1 IHt1 t2 IHt2].
+  - cbn. compose near (dist2 v) on right.
+    rewrite fun_map_map.
+    change (tvar (B := B) (V := term B V)) with
+      (ret (T := term B) (A := term B V)).
+    setoid_rewrite join_ret_term. (* not sure why setoid_ required here *)
+    rewrite fun_map_id.
+    reflexivity.
+  - cbn.
+    rewrite IHbody.
+    rewrite <- ap_map.
+    rewrite map_ap.
+    rewrite app_pure_natural.
+    rewrite map_ap.
+    rewrite map_ap.
+    rewrite app_pure_natural.
+    reflexivity.
+  - cbn.
+    rewrite IHt1.
+    rewrite <- ap_map.
+    rewrite app_pure_natural.
+    rewrite IHt2.
+    rewrite <- ap_map.
+    rewrite map_ap.
+    rewrite app_pure_natural.
+    rewrite map_ap.
+    rewrite map_ap.
+    rewrite app_pure_natural.
+    reflexivity.
+Qed.
+
+
+
+Instance DecoratedTraversableMonadPoly_term:
+  DecoratedTraversableMonadPoly term.
+Proof.
+  constructor.
+  - typeclasses eauto.
+  - typeclasses eauto.
+  - typeclasses eauto.
+  - typeclasses eauto.
+  - reflexivity.
+  - unfold decpoly_ret.
+    intros.
+    ext v.
+    apply decorate_ret_term.
+  - unfold decpoly_join.
+    intros.
+    apply decorate_join_term.
+  - (* dist ret *)
+    admit.
+  - unfold dist2_join.
+    intros.
+    setoid_rewrite dist_join_term.
+    reflexivity.
+  - unfold dist2_decpoly_ci.
+    intros.
+    ext t.
+    now rewrite dist_dec_commute2.
+Abort.
+
