Tealeaves/Examples/LambdaNominal/Equivalence.v
@@ -1,0 +1,355 @@
+From Tealeaves Require Export
+  Examples.LambdaNominal.Syntax
+  Examples.LambdaNominal.Categorical
+  Examples.LambdaNominal.Kleisli
+  Examples.LambdaNominal.Raw
+  Adapters.CategoricalToKleisli.DecoratedTraversableMonadPoly
+  Classes.Categorical.DecoratedTraversableMonadPoly
+  Functors.Subset
+  Functors.Constant
+  Backends.LN.AtomSet
+  Backends.Named.NamedTraditional
+  Simplification.Binddt.
+
+Import DecoratedTraversableMonadPoly.DerivedOperations.
+Import Kleisli.DecoratedTraversableMonadPoly.DerivedOperations.
+Import Kleisli.DecoratedTraversableMonadPoly.
+
+#[local] Generalizable Variables G.
+
+Instance: Kleisli.DecoratedTraversableMonadPoly.DecoratedTraversableMonadPoly term.
+Admitted.
+
+Section rw.
+
+  Context
+    {B1 V1 B2 V2: Type}
+    `{Applicative G}
+    {g: list B1 * B1 -> G B2}
+    {f: list B1 * V1 -> G (term B2 V2)}.
+  Lemma sub_term_spec: forall v,
+      substitute (Substitute := Binddt_Categorical term) g f (tvar v) =
+        substitute (Substitute := Substitute_lambda_term) g f (tvar v).
+  Proof.
+    intros.
+    unfold substitute.
+    unfold Binddt_Categorical.
+    unfold compose.
+    cbn.
+    compose near (f ([], v)).
+    rewrite (fun_map_map).
+    change (join ∘ tvar) with (join ∘ ret (T := term B2) (A := term B2 V2)).
+    rewrite mon_join_ret.
+    rewrite fun_map_id.
+    reflexivity.
+  Qed.
+
+End rw.
+
+
+Lemma test: forall (bs: list name) (t: term name name),
+    substitute (B2 := False) (A2 := False)
+      (G := const (list name)) (T := term) (const [])
+      ((map ret ∘ (fun '(ctx, x) => if get_binding ctx x then [] else [x])) ⦿ bs)
+      t =
+      remove_all bs (fvL t).
+Proof.
+  intros.
+  generalize dependent bs.
+  induction t; intros.
+  - cbn. change (bs ● []) with (bs ● Ƶ).
+    simpl_monoid.
+    remember (get_binding bs v) as R.
+    destruct R.
+    + induction l.
+Admitted.
+
+Lemma FV_fvL : forall (t: term name name),
+    FV term t = fvL t.
+Proof.
+  intros t.
+  induction t.
+  - reflexivity.
+  - unfold FV.
+    unfold mapdtp.
+    unfold MapdtPoly_Substitute.
+    rewrite sub_term_rw2.
+    assert (@const (list name * name) (list name) [] ⦿ [b] =
+              (const (A := list name * name) (@nil name))).
+    { ext x. reflexivity.}
+    setoid_rewrite H.
+    rewrite test.
+    repeat simplify_applicative_const.
+    simplify_monoid_units.
+    cbn.
+    reflexivity.
+  - cbn. rewrite IHt1.
+    rewrite IHt2.
+    reflexivity.
+Qed.
+
+(*
+Section rw.
+
+  Context (x: name) (u: term name name).
+
+  Lemma subst_term_rw1: forall (v: name),
+      Named.subst term x u (tvar v) =
+        if (v == x) then u else (tvar v).
+  Proof.
+    reflexivity.
+  Qed.
+  Lemma subst_conflicts_rw1: forall top (v: name),
+      subst_conflicts term top x u (tvar v) =
+        if (v == x) then u else (tvar v).
+  Proof.
+    reflexivity.
+  Qed.
+
+  Lemma subst_conflicts_rw2: forall (top: list name) (b: name) (t: term name name),
+      subst_conflicts term top x u (lam b t) =
+        lam (rename_binder_local top ([], b))
+          (DecoratedTraversableMonadPoly.substitute (G := fun A => A)
+             (rename_binder_local top ⦿ [b])
+             (subst_local top x u ⦿ [b]) t).
+  Proof.
+    intros.
+    reflexivity.
+  Qed.
+
+  Lemma subst_conflicts_rw3: forall (top: list name) (t1 t2: term name name),
+      subst_conflicts term top x u (tap t1 t2) =
+        tap (subst_conflicts term top x u t1) (subst_conflicts term top x u t2).
+  Proof.
+    reflexivity.
+  Qed.
+End rw.
+*)
+
+
+Section rw.
+
+  Context
+    (top: list name)
+    (x: name) (fv_u: list name) (u: term name name).
+
+  Lemma subst_top_rw1: forall (v: name),
+      subst_top top x fv_u u (tvar v) =
+        if (v == x) then u else (tvar v).
+  Proof.
+    reflexivity.
+  Qed.
+
+  Lemma subst_top_rw2: forall (b: name) (t: term name name),
+      subst_top top x (fv_u) u (lam b t) =
+        lam (rename_binder_local top x fv_u ([], b))
+          (substitute (G := fun A => A)
+             (rename_binder_local top x fv_u ⦿ [b])
+             (subst_local top x fv_u u ⦿ [b]) t).
+  Proof.
+    intros.
+    unfold subst_top.
+    rewrite sub_term_rw2.
+    repeat simplify_applicative_I.
+    reflexivity.
+  Qed.
+
+  Lemma subst_top_rw3: forall (top: list name) (t1 t2: term name name),
+      subst_top top x fv_u u (tap t1 t2) =
+        tap (subst_top top x fv_u u t1) (subst_top top x fv_u u t2).
+  Proof.
+    reflexivity.
+  Qed.
+
+End rw.
+
+
+
+
+Import ContainerFunctor.Notations.
+
+Lemma rename_binder_kill2: forall top x fv_u,
+    rename_binder_local top x fv_u ([], x) = x.
+Proof.
+  intros.
+  cbn.
+  destruct_eq_args x x.
+Qed.
+
+Lemma rename_binder_kill: forall top x fv_u l ctx v,
+    x ∈ l ->
+    (rename_binder_local top x fv_u ⦿ l) (ctx, v) = v.
+Proof.
+  intros.
+  change (rename_binder_local top x fv_u (l ++ ctx, v) = v).
+  unfold rename_binder_local.
+  remember (SmartAtom.name_inb x (l ++ ctx)).
+  destruct b.
+  + reflexivity.
+  + false.
+    symmetry in Heqb.
+    rewrite SmartAtom.name_inb_iff_false in Heqb.
+    rewrite element_of_list_app in Heqb.
+    intuition.
+Qed.
+
+Lemma subst_local_kill: forall top x fv_u u l ctx v,
+    x ∈ l ->
+    (subst_local top x fv_u u ⦿ l) (ctx, v) = tvar v.
+Proof.
+  intros.
+  change (subst_local top x fv_u u (l ++ ctx, v) = tvar v).
+  unfold subst_local.
+  remember (SmartAtom.name_inb x (l ++ ctx)).
+  destruct b.
+  + reflexivity.
+  + false.
+    symmetry in Heqb.
+    rewrite SmartAtom.name_inb_iff_false in Heqb.
+    rewrite element_of_list_app in Heqb.
+    intuition.
+Qed.
+
+
+Lemma kill:
+  forall (top fv_u: list name) (any: list name) (x: name) (t u: term name name),
+    x ∈ any ->
+    substitute (T := term) (G := fun A => A)
+      (rename_binder_local top x fv_u ⦿ any)
+      (subst_local top x fv_u u ⦿ any) t = t.
+Proof.
+  intros.
+  change t with (id t) at 2.
+  rewrite <- (kdtmp_substitute1 (T := term) (B := name) (A := name)).
+  fequal.
+  - ext (ctx, v).
+    now apply rename_binder_kill.
+  - ext (ctx, v).
+    now apply subst_local_kill.
+Qed.
+
+Lemma substSmart_equiv:
+  forall (top: list name) (x: name) (u: term name name),
+    subst_top top x (FV term u) u =
+      substF top x u.
+Proof.
+  intros. ext t. induction t.
+  - rewrite subst_top_rw1.
+    rewrite substF_rw1.
+    reflexivity.
+  - rewrite subst_top_rw2.
+    rewrite substF_rw2.
+    destruct_eq_args b x.
+    + fequal.
+      apply rename_binder_kill2.
+      apply kill.
+      now simpl_list.
+    +
+      rewrite FV_fvL.
+      remember ((SmartAtom.name_inb b (fvL u))) as rem.
+      destruct rem.
+      * fequal.
+        { cbn.
+          destruct_eq_args x b.
+          rewrite <- Heqrem.
+          reflexivity.
+        }
+
+
+
+
+      unfold rename_binder_local.
+      assert (SmartAtom.name_inb x [] = false).
+      { reflexivity. }
+      rewrite H. destruct_eq_args x b.
+      rewrite FV_fvL.
+      remember ((SmartAtom.name_inb b (fvL u))) as rem.
+      destruct rem.
+      * fequal.
+        {
+        }
+        {
+          admit.
+        }
+      * cbn.
+        admit.
+  - rewrite subst_top_rw3.
+    rewrite substF_rw3.
+    rewrite IHt1.
+    rewrite IHt2.
+    reflexivity.
+Admitted.
+
+Corollary substSmart_equiv_truly:
+  forall (x: name) (u: term name name) t,
+    substSmart x u t =
+      Raw.subst x u t.
+Proof.
+  intros.
+  unfold substSmart.
+  unfold Raw.subst.
+  rewrite FV_fvL.
+  rewrite FV_fvL.
+  apply substSmart_equiv.
+Qed.
+
+
+
+
+
+
+
+
+
+
+
+
+
+
+
+
+
+
+
+
+
+
+
+
+
+
+
+  (*
+  Lemma subst_conflicts_rw2: forall (top: list name) (b: name) (t: term name name),
+      subst_conflicts term top x u (lam b t) =
+        lam (rename_binder_local top ([], b))
+          (DecoratedTraversableMonadPoly.substitute (G := fun A => A)
+             (rename_binder_local top ⦿ [b])
+             (subst_local top x u ⦿ [b]) t).
+  Proof.
+    intros.
+    unfold subst.
+    unfold subst_conflicts.
+    unfold DecoratedTraversableMonadPoly.substitute.
+    unfold Binddt_Categorical.
+    unfold compose at 1 2 3 4.
+    rewrite dec_term_rw2.
+    rewrite map2_term_rw2.
+    rewrite dist2_unit.
+    unfold id.
+    unfold_ops @Map_I.
+    rewrite join_term_rw2.
+    fequal.
+    change (fun x : term name (term name name) => x) with
+      (@id (term name (term name name))).
+    change (?f ∘ id) with f.
+    compose near ([b], decp t) on left.
+    compose near (decp t) on left.
+    rewrite (map2_shift2_preincr
+               (g := (rename_binder_local top))
+               (f := (subst_local top x u))
+               (w := [b])).
+
+    reflexivity.
+  Qed.
+  *)
