Tealeaves/Examples/LambdaNominal/Raw.v
@@ -1,0 +1,146 @@
+From Tealeaves Require Export
+  Examples.LambdaNominal.Syntax
+  Functors.Subset
+  Backends.LN.AtomSet
+  Backends.Named.Names.
+
+Require Coq.funind.Recdef.  (* Needed for Function *)
+
+
+Import Early.Subset.Notations.
+
+Fixpoint fv (t: term name name): subset name :=
+  match t with
+  | tvar v => {{ v }}
+  | tap t1 t2 => fv t1 ∪ fv t2
+  | lam b t => fun v => (fv t v) /\  (v <> b)
+  end.
+
+Fixpoint remove (x: name) (l: list name) : list name :=
+  match l with
+  | nil => nil
+  | cons y rest =>
+      if x == y then remove x rest else cons y (remove x rest)
+  end.
+
+Fixpoint remove_all (xs: list name) (l: list name) : list name :=
+  match xs with
+  | nil => l
+  | cons y rest =>
+      remove_all rest (remove y l)
+  end.
+
+Fixpoint fvL (t: term name name): list name :=
+  match t with
+  | tvar v => [ v ]
+  | tap t1 t2 => fvL t1 ++ fvL t2
+  | lam b t => remove b (fvL t)
+  end.
+
+Fixpoint rename (x: name) (y: name) (t: term name name): term name name :=
+  match t with
+  | tvar v => if x == v then tvar y else tvar v
+  | tap t1 t2 => tap (rename x y t1) (rename x y t2)
+  | lam b t => if b == x then lam b t
+              else lam b (rename x y t)
+  end.
+
+
+(* Depth function for well-founded recursion *)
+Fixpoint depth (t : term name name) : nat :=
+  match t with
+  | tvar _ => 0
+  | lam b t => S (depth t)
+  | tap t1 t2 => S (max (depth t1) (depth t2))
+  end.
+
+(* Well-founded measure for lexicographic ordering *)
+Definition term_measure (t : term name name) : nat := depth t.
+
+Lemma depth_rename_eq:
+  forall (x y : name) (t : term name name),
+    depth (rename x y t) = depth t.
+Proof.
+  intros.
+  induction t.
+  - cbn. destruct_eq_args x v.
+  - cbn. destruct_eq_args x b.
+    cbn.
+    rewrite IHt.
+    reflexivity.
+  - cbn. lia.
+Qed.
+
+(* Capture-avoiding substitution with well-founded recursion *)
+Function substF (l: list name)
+  (x : name) (u : term name name)
+  (t : term name name)
+  {measure term_measure t}
+  : term name name :=
+  match t with
+  | tvar y => if y == x then u else tvar y
+  | tap t1 t2 =>
+      tap (substF l x u t1) (substF l x u t2)
+  | lam b t =>
+      if b == x then lam b t
+      else if SmartAtom.name_inb b (fvL u)
+           then let z := (fresh (l ++ [b]): name) in
+                lam z (substF (l ++ [z]) x u (rename x z t))
+           else lam b (substF (l ++ [b]) x u t)
+  end.
+Proof.
+  all: unfold term_measure.
+  - intros.
+    rewrite depth_rename_eq.
+    cbn. lia.
+  - intros.
+    cbn.
+    lia.
+  - intros.
+    cbn.
+    lia.
+  - intros.
+    cbn.
+    lia.
+Qed.
+
+Section rw.
+
+  Context {l: list name} {x: name} {u: term name name}.
+
+  Lemma substF_rw1: forall v,
+      substF l x u (tvar v) = (if v == x then u else tvar v).
+  Proof.
+    intros.
+    rewrite substF_equation.
+    reflexivity.
+  Qed.
+
+  Lemma substF_rw2: forall b t,
+      substF l x u (lam b t) =
+        (if b == x
+   then (λ) b t
+   else
+    if SmartAtom.name_inb b (fvL u)
+    then
+     (λ) (fresh (l ++ [b]))
+       (substF (l ++ [fresh (l ++ [b])]) x u (rename x (fresh (l ++ [b])) t))
+    else (λ) b (substF (l ++ [b]) x u t)).
+  Proof.
+    intros.
+    rewrite substF_equation.
+    reflexivity.
+  Qed.
+
+  Lemma substF_rw3: forall t1 t2,
+      substF l x u (tap t1 t2) = tap (substF l x u t1) (substF l x u t2).
+  Proof.
+    intros.
+    rewrite substF_equation.
+    reflexivity.
+  Qed.
+
+End rw.
+
+Definition subst (x : name) (u : term name name) (t : term name name) :=
+  substF (fvL t ++ fvL u) x u t.
